feat(le‑fs): shadow‑lane sampler refactor with stable theorem names; no axioms added; checker clean

docs/03-formal-verification/easycrypt/le/LEFsProgrammingSurface.ec
@@ -1,9 +1,11 @@
 require import QssmTypes.
 require import AllCore Distr.
+require import List.
 require import Real.
 require import SDist.
 require import StdOrder.
 require import LESurface.
+require BudgetParameters.
 
 (*---*) import RealOrder.
 
@@ -268,6 +270,29 @@ have Hhalf : 0%r <= (1%r / 2%r) * epsilon_le by smt().
 exact Hhalf.
 qed.
 
+lemma A_LE_fs_hidden_state_update_sdist_le_budget :
+  forall (x : qssm_public_input) (s : seed) (D : distinguisher),
+    le_real_view_distribution_defined x s =>
+    le_sim_view_distribution_defined x s =>
+    le_fs_programming_hiding_bound x s D =>
+    sdist (d_le_pre_fs_hidden_programming_state x s)
+      (dmap (d_le_pre_fs_hidden_programming_state x s)
+        le_fs_hidden_programming_state_update)
+      <= BudgetParameters.epsilon_le_fs.
+proof.
+move=> x s D _ _ _.
+have Hmap :
+  dmap (d_le_pre_fs_hidden_programming_state x s)
+    le_fs_hidden_programming_state_update =
+  dmap (d_le_pre_fs_hidden_programming_state x s)
+    (fun (st : le_fs_hidden_programming_state) => st).
+  apply eq_dmap_in=> st _ /=.
+  exact (le_fs_hidden_state_update_id st).
+rewrite Hmap dmap_id sdistdd.
+rewrite /BudgetParameters.epsilon_le_fs.
+by [].
+qed.
+
 lemma A_LE_fs_hidden_material_programming_sdist_bound :
   forall (x : qssm_public_input) (s : seed) (D : distinguisher),
     le_real_view_distribution_defined x s =>
@@ -281,6 +306,20 @@ proof.
 move=> x s D Hr Hs Hfs Heps.
 rewrite /d_le_post_fs_hidden_programming_state.
 exact (A_LE_fs_hidden_state_update_sdist_bound x s D Hr Hs Hfs Heps).
+qed.
+
+lemma A_LE_fs_hidden_material_programming_sdist_le_budget :
+  forall (x : qssm_public_input) (s : seed) (D : distinguisher),
+    le_real_view_distribution_defined x s =>
+    le_sim_view_distribution_defined x s =>
+    le_fs_programming_hiding_bound x s D =>
+    sdist (d_le_pre_fs_hidden_programming_state x s)
+      (d_le_post_fs_hidden_programming_state x s)
+      <= BudgetParameters.epsilon_le_fs.
+proof.
+move=> x s D Hr Hs Hfs.
+rewrite /d_le_post_fs_hidden_programming_state.
+exact (A_LE_fs_hidden_state_update_sdist_le_budget x s D Hr Hs Hfs).
 qed.
 
 lemma A_LE_fs_programming_sampler_sdist_bound :
@@ -310,6 +349,32 @@ exact (ler_trans _ _ _ Hmap
   (A_LE_fs_hidden_material_programming_sdist_bound x s D Hr Hs Hfs Heps)).
 qed.
 
+lemma A_LE_fs_programming_sampler_sdist_le_budget :
+  forall (x : qssm_public_input) (s : seed) (D : distinguisher),
+    le_real_view_distribution_defined x s =>
+    le_sim_view_distribution_defined x s =>
+    le_fs_programming_hiding_bound x s D =>
+    sdist (d_le_pre_fs_programming_view x s)
+      (d_le_post_fs_programmed_view x s)
+      <= BudgetParameters.epsilon_le_fs.
+proof.
+move=> x s D Hr Hs Hfs.
+rewrite d_le_pre_fs_programming_view_matches_hidden_state_projection.
+rewrite d_le_post_fs_programmed_view_matches_hidden_state_projection.
+have Hmap :
+  sdist (dmap (d_le_pre_fs_hidden_programming_state x s)
+          le_fs_observable_of_hidden_programming_state)
+        (dmap (d_le_post_fs_hidden_programming_state x s)
+          le_fs_observable_of_hidden_programming_state)
+    <= sdist (d_le_pre_fs_hidden_programming_state x s)
+         (d_le_post_fs_hidden_programming_state x s).
+  exact (sdist_dmap (d_le_pre_fs_hidden_programming_state x s)
+    (d_le_post_fs_hidden_programming_state x s)
+    le_fs_observable_of_hidden_programming_state).
+exact (ler_trans _ _ _ Hmap
+  (A_LE_fs_hidden_material_programming_sdist_le_budget x s D Hr Hs Hfs)).
+qed.
+
 lemma le_fs_surrogate_matches_programmed_view :
   forall (x : qssm_public_input) (s : seed),
     d_le_post_fs_programmed_view x s =
@@ -331,6 +396,244 @@ move=> obs.
 rewrite /le_fs_surrogate_transform /le_fs_view_surrogate.
 rewrite /le_commitment_coeffs /le_t_coeffs /le_z_coeffs.
 rewrite /le_challenge_seed_obs /le_programmed_query_digest_obs.
+by [].
+qed.
+
+type le_fs_shadow_hidden_material = {
+  lefshm_query_row : le_fs_query_row;
+  lefshm_pre_query_material : le_query_material;
+  lefshm_semantic_post_query_material : le_query_material;
+  lefshm_programmed_response : le_fs_programmed_response_carrier;
+  lefshm_bad_flag : bool;
+}.
+
+type le_fs_shadow_state = {
+  lefss_pre_observable : le_transcript_observable;
+  lefss_post_observable : le_transcript_observable;
+  lefss_hidden_material : le_fs_shadow_hidden_material;
+}.
+
+op le_fs_shadow_programming_log_of_observable
+  (obs : le_transcript_observable) : digest list =
+  [le_challenge_seed_obs obs; le_programmed_query_digest_obs obs].
+
+op le_fs_shadow_semantic_post_query_material_of_observable
+  (obs : le_transcript_observable) : le_query_material =
+  {| leqm_row_challenge_seed = le_challenge_seed_obs obs;
+     leqm_row_programmed_query_digest = le_programmed_query_digest_obs obs;
+     leqm_programmed_response_digest = le_programmed_query_digest_obs obs;
+     leqm_programming_log = le_fs_shadow_programming_log_of_observable obs;
+     leqm_bad_flag = false |}.
+
+op le_fs_shadow_hidden_material_of_observable
+  (obs : le_transcript_observable) : le_fs_shadow_hidden_material =
+  {| lefshm_query_row = le_fs_query_row_of_observable obs;
+     lefshm_pre_query_material = le_fs_query_material_obs obs;
+     lefshm_semantic_post_query_material =
+       le_fs_shadow_semantic_post_query_material_of_observable obs;
+     lefshm_programmed_response = le_fs_programmed_response_of_observable obs;
+     lefshm_bad_flag = false |}.
+
+op le_fs_shadow_post_of_observable
+  (obs : le_transcript_observable) (hm : le_fs_shadow_hidden_material) :
+  le_transcript_observable =
+  hm.`lefshm_programmed_response.`lefspc_programmed_view.
+
+op le_fs_shadow_state_of_observable
+  (obs : le_transcript_observable) : le_fs_shadow_state =
+  let hm = le_fs_shadow_hidden_material_of_observable obs in
+  {| lefss_pre_observable = obs;
+     lefss_post_observable = le_fs_shadow_post_of_observable obs hm;
+     lefss_hidden_material = hm |}.
+
+op le_fs_shadow_pre_observable
+  (st : le_fs_shadow_state) : le_transcript_observable =
+  st.`lefss_pre_observable.
+
+op le_fs_shadow_post_observable
+  (st : le_fs_shadow_state) : le_transcript_observable =
+  st.`lefss_post_observable.
+
+op le_fs_shadow_bad_event
+  (st : le_fs_shadow_state) : bool =
+  st.`lefss_hidden_material.`lefshm_bad_flag.
+
+op d_le_fs_shadow_coupled_state
+  (x : qssm_public_input) (s : seed) : le_fs_shadow_state distr =
+  dmap (d_le_pre_fs_programming_view x s)
+    le_fs_shadow_state_of_observable.
+
+op d_le_fs_shadow_pre_marginal
+  (x : qssm_public_input) (s : seed) : le_transcript_observable distr =
+  dmap (d_le_fs_shadow_coupled_state x s)
+    le_fs_shadow_pre_observable.
+
+op d_le_fs_shadow_post_marginal
+  (x : qssm_public_input) (s : seed) : le_transcript_observable distr =
+  dmap (d_le_fs_shadow_coupled_state x s)
+    le_fs_shadow_post_observable.
+
+op le_fs_shadow_failure_probability
+  (x : qssm_public_input) (s : seed) =
+  mu (d_le_fs_shadow_coupled_state x s)
+    le_fs_shadow_bad_event.
+
+lemma le_fs_shadow_post_of_observable_matches_surrogate
+  (obs : le_transcript_observable) :
+  (le_fs_shadow_state_of_observable obs).`lefss_post_observable =
+  le_fs_surrogate_transform obs.
+proof.
+rewrite /le_fs_shadow_state_of_observable.
+rewrite /le_fs_shadow_post_of_observable.
+rewrite /le_fs_shadow_hidden_material_of_observable.
+by rewrite /le_fs_programmed_response_of_observable.
+qed.
+
+lemma le_fs_shadow_post_observable_preserves_visible_fields
+  (obs : le_transcript_observable) :
+  le_commitment_coeffs ((le_fs_shadow_state_of_observable obs).`lefss_post_observable) =
+    le_commitment_coeffs obs /\
+  le_t_coeffs ((le_fs_shadow_state_of_observable obs).`lefss_post_observable) =
+    le_t_coeffs obs /\
+  le_z_coeffs ((le_fs_shadow_state_of_observable obs).`lefss_post_observable) =
+    le_z_coeffs obs /\
+  le_challenge_seed_obs ((le_fs_shadow_state_of_observable obs).`lefss_post_observable) =
+    le_challenge_seed_obs obs /\
+  le_programmed_query_digest_obs ((le_fs_shadow_state_of_observable obs).`lefss_post_observable) =
+    le_programmed_query_digest_obs obs.
+proof.
+rewrite (le_fs_shadow_post_of_observable_matches_surrogate obs).
+exact (le_fs_programming_preserves_shape_lower obs).
+qed.
+
+lemma le_fs_shadow_bad_event_current_model
+  (obs : le_transcript_observable) :
+  le_fs_shadow_bad_event (le_fs_shadow_state_of_observable obs) = false.
+proof.
+rewrite /le_fs_shadow_bad_event /le_fs_shadow_state_of_observable.
+by rewrite /le_fs_shadow_hidden_material_of_observable.
+qed.
+
+lemma d_le_fs_shadow_pre_marginal_matches_pre_programming_view :
+  forall (x : qssm_public_input) (s : seed),
+    d_le_fs_shadow_pre_marginal x s = d_le_pre_fs_programming_view x s.
+proof.
+move=> x s.
+rewrite /d_le_fs_shadow_pre_marginal /d_le_fs_shadow_coupled_state.
+rewrite (dmap_comp le_fs_shadow_state_of_observable
+  le_fs_shadow_pre_observable
+  (d_le_pre_fs_programming_view x s)).
+have Hmap :
+  dmap (d_le_pre_fs_programming_view x s)
+    (le_fs_shadow_pre_observable \o le_fs_shadow_state_of_observable) =
+  dmap (d_le_pre_fs_programming_view x s)
+    (fun (obs : le_transcript_observable) => obs).
+  apply eq_dmap_in=> obs _ /=.
+  by rewrite /le_fs_shadow_pre_observable /le_fs_shadow_state_of_observable /(\o).
+rewrite Hmap.
+by rewrite dmap_id.
+qed.
+
+lemma d_le_fs_shadow_pre_marginal_matches_post_rejection_view :
+  forall (x : qssm_public_input) (s : seed),
+    d_le_fs_shadow_pre_marginal x s = d_le_post_rejection_view x s.
+proof.
+move=> x s.
+rewrite d_le_fs_shadow_pre_marginal_matches_pre_programming_view.
+by rewrite /d_le_pre_fs_programming_view.
+qed.
+
+lemma d_le_fs_shadow_post_marginal_matches_programmed_view :
+  forall (x : qssm_public_input) (s : seed),
+    d_le_fs_shadow_post_marginal x s = d_le_post_fs_programmed_view x s.
+proof.
+move=> x s.
+rewrite /d_le_fs_shadow_post_marginal /d_le_fs_shadow_coupled_state.
+rewrite (dmap_comp le_fs_shadow_state_of_observable
+  le_fs_shadow_post_observable
+  (d_le_pre_fs_programming_view x s)).
+have Hmap :
+  dmap (d_le_pre_fs_programming_view x s)
+    (le_fs_shadow_post_observable \o le_fs_shadow_state_of_observable) =
+  dmap (d_le_pre_fs_programming_view x s)
+    le_fs_surrogate_transform.
+  apply eq_dmap_in=> obs _ /=.
+  rewrite /le_fs_shadow_post_observable /(\o).
+  exact (le_fs_shadow_post_of_observable_matches_surrogate obs).
+rewrite Hmap.
+by rewrite /d_le_post_fs_programmed_view.
+qed.
+
+lemma d_le_fs_shadow_post_marginal_matches_sim_view :
+  forall (x : qssm_public_input) (s : seed),
+    d_le_fs_shadow_post_marginal x s = d_le_sim_view x s.
+proof.
+move=> x s.
+rewrite d_le_fs_shadow_post_marginal_matches_programmed_view.
+by rewrite /d_le_post_fs_programmed_view /d_le_pre_fs_programming_view
+  /d_le_sim_view /le_fs_surrogate_transform.
+qed.
+
+lemma le_fs_surrogate_transform_id
+  (obs : le_transcript_observable) :
+  le_fs_surrogate_transform obs = obs.
+proof.
+case: obs=> ccoeffs tcoeffs zcoeffs cseed pqdig qmat payload /=.
+by rewrite /le_fs_surrogate_transform /le_fs_view_surrogate
+  /le_fs_program_query_material.
+qed.
+
+lemma d_le_fs_shadow_pre_post_marginals_equal :
+  forall (x : qssm_public_input) (s : seed),
+    d_le_fs_shadow_pre_marginal x s = d_le_fs_shadow_post_marginal x s.
+proof.
+move=> x s.
+rewrite d_le_fs_shadow_pre_marginal_matches_pre_programming_view.
+rewrite d_le_fs_shadow_post_marginal_matches_programmed_view.
+rewrite /d_le_post_fs_programmed_view.
+have Hmap :
+  dmap (d_le_pre_fs_programming_view x s) le_fs_surrogate_transform =
+  dmap (d_le_pre_fs_programming_view x s)
+    (fun (obs : le_transcript_observable) => obs).
+  apply eq_dmap_in=> obs _ /=.
+  exact (le_fs_surrogate_transform_id obs).
+rewrite Hmap.
+by rewrite dmap_id.
+qed.
+
+lemma le_fs_shadow_failure_probability_zero :
+  forall (x : qssm_public_input) (s : seed),
+    le_fs_shadow_failure_probability x s = 0%r.
+proof.
+move=> x s.
+rewrite /le_fs_shadow_failure_probability /d_le_fs_shadow_coupled_state.
+rewrite /d_le_pre_fs_programming_view /d_le_post_rejection_view.
+rewrite /d_le_real_view /d_le_real_execution_view /le_post_rejection_surrogate.
+rewrite dmap_dunit dmap_dunit dunitE /=.
+rewrite /le_fs_shadow_bad_event /le_fs_shadow_state_of_observable.
+by rewrite /le_fs_shadow_hidden_material_of_observable.
+qed.
+
+lemma A_LE_fs_shadow_sdist_le_failure_probability :
+  forall (x : qssm_public_input) (s : seed),
+    sdist (d_le_fs_shadow_pre_marginal x s)
+      (d_le_fs_shadow_post_marginal x s)
+      <= le_fs_shadow_failure_probability x s.
+proof.
+move=> x s.
+rewrite (d_le_fs_shadow_pre_post_marginals_equal x s).
+rewrite sdistdd.
+rewrite (le_fs_shadow_failure_probability_zero x s).
+by [].
+qed.
+
+lemma A_LE_fs_shadow_failure_probability_le_budget :
+  forall (x : qssm_public_input) (s : seed),
+    le_fs_shadow_failure_probability x s <= BudgetParameters.epsilon_le_fs.
+proof.
+move=> x s.
+rewrite (le_fs_shadow_failure_probability_zero x s).
+rewrite /BudgetParameters.epsilon_le_fs.
 by [].
 qed.
 
